porting code to ExtLib 0.2

src/Cps.v
@@ -1,11 +1,18 @@
-Require Import Lambda.
-Require Import ZArith String List Bool.
-Require Import ExtLib.Monad.Monad.
-Require Import ExtLib.Monad.OptionMonad ExtLib.Monad.StateMonad.
-Require Import ExtLib.Monad.Folds.
+Require Import CoqCompile.Lambda CoqCompile.Env.
 Require Import ExtLib.Data.Strings.
-Require Import ExtLib.Decidables.Decidable.
+Require Import ZArith String List Bool.
+Require Import ExtLib.Structures.Monads.
+Require Import ExtLib.Data.Monads.StateMonad.
+Require Import ExtLib.Data.Monads.OptionMonad.
+Require Import ExtLib.Structures.Reducible.
+Require Import ExtLib.Structures.Folds.
+Require Import ExtLib.Data.Strings.
+Require Import ExtLib.Data.Lists.
+Require Import ExtLib.Core.RelDec.
+Require Import ExtLib.Core.ZDecidables.
+Require Import ExtLib.Core.PosDecidables.
 Require Import ExtLib.Tactics.Consider.
+
 
 Set Implicit Arguments.
 Set Strict Implicit.
@@ -16,7 +23,6 @@ Set Strict Implicit.
 Module CPS.
   Import MonadNotation. 
   Local Open Scope monad_scope.
-  Definition var := Lambda.var.
   Definition constructor := Lambda.constructor.
   Definition env_t := Lambda.env_t.
 
@@ -77,131 +83,6 @@ Module CPS.
         will either be a [Fn_d] or else a [Prim_d _ MkTuple_p]. *)
   | Rec_d : list decl -> decl.
 
-  (** Pretty printing CPS expressions *)
-  Section PP.
-    Local Open Scope string_scope.
-
-    Definition pos2string(p:positive) := LambdaNotation.nat2string (Pos.to_nat p).
-    Fixpoint spaces (n:nat) : string :=
-      match n with
-        | 0 => ""
-        | S n => " " ++ (spaces n)
-      end.
-
-    Definition emit (s:string) : state (list string) unit :=
-      sofar <- get ; put (s::sofar).
-    
-    Fixpoint indent (n:nat) : state (list string) unit :=
-      match n with
-        | 0 => ret tt
-        | S n => emit " " ;; indent n
-      end.
-
-    Fixpoint emit_list{A}(f:A->string)(vs:list A) : state (list string) unit :=
-      match vs with
-        | nil => ret tt
-        | v::nil => emit (f v)
-        | v::vs => emit (f v) ;; emit "," ;; emit_list f vs
-      end.
-
-    Definition newline : string := (String (Ascii.ascii_of_nat 10) EmptyString).
-
-    Section ITER.
-      Context {S A:Type}.
-      Variable f : A -> state S unit.
-      
-      Fixpoint iter (xs:list A) : state S unit :=
-        match xs with
-          | nil => ret tt
-          | h::t => f h ;; iter t
-        end.
-    End ITER.
-
-    Definition z2string(x:Z) : string := 
-      match x with 
-        | Z0 => "0"
-        | Zpos p => pos2string p
-        | Zneg p => "-" ++ (pos2string p)
-      end.
-    Definition op2string (v:op) : string := 
-      match v with 
-        | Var_o x => x
-        | Con_o c => "Con(" ++ c ++ ")"
-        | Int_o i => z2string i
-      end.
-    Definition pat2string (p:pattern) : string := 
-      match p with 
-        | Int_p i => z2string i
-        | Con_p c => c
-      end.
-    Definition primop2string (p:primop) : string := 
-      match p with 
-        | Eq_p => "eq?"
-        | Neq_p => "neq?"
-        | Lt_p => "lt?"
-        | Lte_p => "lte?"
-        | Ptr_p => "ptr?"
-        | Plus_p => "+"
-        | Minus_p => "-"
-        | Times_p => "*"
-        | Proj_p => "#"
-        | MkTuple_p => "mkTuple"
-      end.
-
-     Fixpoint emitexp (n:nat)(e:exp) : state (list string) unit := 
-       emit newline ;; indent n ;;
-       match e with 
-         | App_e v vs => emit (op2string v) ;; emit "(" ;; emit_list op2string vs ;; emit ")" 
-         | Let_e d e => 
-           emit "let ";; emitdecl false (2+n) d ;; emitexp (2+n) e 
-         | Switch_e v arms def => 
-           emit "switch ";; emit (op2string v) ;; emit " with" ;; 
-           iter (fun (p: pattern * exp) => 
-             emit newline ;; indent n ;; emit "| ";; emit (pat2string (fst p)) ;; emit " => ";; 
-             emitexp (2+n) (snd p)) arms ;;
-           match def with 
-             | None => ret tt 
-             | Some e => emit newline ;; indent n ;; emit "| _ => " ;; emitexp (2+n) e
-           end ;;
-           emit newline ;; indent n ;; emit "end"
-         | Halt_e o => emit "HALT " ;; emit (op2string o)
-       end
-     with emitdecl (inrec:bool)(n:nat)(d:decl) : state (list string) unit := 
-       let emit_sep : state (list string) unit := if inrec then emit " and" else emit " in" in 
-       match d with 
-         | Op_d x v => 
-           emit x ;; emit " = " ;; emit (op2string v) ;; emit_sep 
-         | Prim_d x p vs => 
-           emit x ;; emit " = " ;; emit (primop2string p) ;; emit "(" ;; 
-           emit_list op2string vs ;; emit ")" ;; emit_sep 
-         | Fn_d f xs e => 
-           emit f ;; emit "(" ;; emit_list (fun x => x) xs ;; emit ") = " ;; 
-           emitexp (2+n) e ;; emit_sep 
-         | Rec_d ds => 
-           emit "rec ";; 
-           let iter_sep := 
-             fix iter_sep(ds:list decl) : state (list string) unit := 
-             match ds with 
-               | nil => emit_sep
-               | d::nil => emitdecl inrec (2+n) d 
-               | d::ds => emitdecl true (2+n) d ;; emit newline ;; indent n ;; iter_sep ds 
-             end
-             in
-             iter_sep ds
-       end.
-
-     Definition exp2string(e:exp) : string := 
-       List.fold_left (fun x y => y ++ x) (snd (runState (emitexp 0 e) nil)) "".
-  End PP.
-
-  Global Instance RelDec_Z_eq : RelDec (@eq Z) := 
-  { rel_dec := Zeq_bool }.
-
-  Global Instance RelDecCorrect_Z_eq : RelDec_Correct RelDec_Z_eq.
-  Proof.
-    constructor. intros.  generalize (Zeq_is_eq_bool x y). simpl. intros. tauto.
-  Qed.
-
   Global Instance RelDec_primop_eq : RelDec (@eq primop) := 
   { rel_dec := fun x y =>
     match x , y with
@@ -220,7 +101,7 @@ Module CPS.
 
   Global Instance RelDecCorrect_primop_eq : RelDec_Correct RelDec_primop_eq.
   Proof.
-    constructor. destruct x; destruct y; simpl; split; intros; subst; try congruence.
+    constructor; destruct x; destruct y; simpl rel_dec; split; intros; subst; try congruence.
   Qed.
 
   Global Instance RelDec_op_eq : RelDec (@eq op) :=
@@ -233,406 +114,119 @@ Module CPS.
 
   Global Instance RelDecCorrect_op_eq : RelDec_Correct RelDec_op_eq.
   Proof.
-    constructor. destruct x; destruct y; simpl; split; intros; subst; try congruence ; 
-    try ((consider (string_dec v v0) || consider (string_dec c c0))) ; intros ; subst; 
-      try congruence ; generalize (Zeq_is_eq_bool z z0) ; intros ;destruct H0. rewrite (H1 H). auto.
-    injection H ; intros ; subst. auto.
+    Opaque Env.RelDec_var_eq RelDec_zeq.
+    constructor. destruct x; destruct y; simpl; unfold eq_dec; try congruence; 
+    try rewrite rel_dec_correct; intuition try congruence.
+    consider (string_dec c c0); intuition congruence.
+    consider (string_dec c c0); intuition congruence.
+    Transparent Env.RelDec_var_eq RelDec_zeq.
   Qed.
 
-  (** returns the function name f if [fun x => e] is a simple eta expansion of the form
-     [fun x => f x]. *)
-  Definition match_eta (x:var) (e:exp) : option op := 
-    match e with 
-      | App_e op1 ((Var_o y)::nil) => 
-        if eq_dec y x then Some op1 else None
-      | _ => None
-    end.
-  
-  Fixpoint eq_vars_ops (xs:list var) (vs:list op) : bool := 
-    match xs, vs with 
-      | nil, nil => true
-      | x::xs, (Var_o y)::vs => eq_dec x y && eq_vars_ops xs vs
-      | _, _ => false
-    end.
-  
-  (** similar to the above, but for the general case of [fun (x1,...,xn) => e] being an
-     eta-expansion of [fun (x1,...,xn) => f(x1,...,xn)]. *)
-  Definition match_etas (xs:list var) (e:exp) : option op := 
-    match e with 
-      | App_e op1 ys =>
-        if eq_vars_ops xs ys then Some op1 else None
-      | _ => None
-    end.
-  
-  (** Let-bind [xi] to [#i v] for the expression [e].  This is used in the compilation
-      of pattern matching below. *)
-  Fixpoint bind_proj(v:op)(xs:list var)(offset:Z)(e:exp) : exp := 
-    match xs with 
-      | nil => e
-      | x::xs => Let_e (Prim_d x Proj_p ((Int_o offset)::v::nil)) (bind_proj v xs (1+offset) e)
-    end.
-  
-  (** Partition pattern matching arms into three classes -- (1) those that are matching on 
-     nullary constructors, (2) those matching on nary constructors for n > 0, (3) a default
-     pattern that matches anything.  Used in match compilation below. *)
-  Fixpoint partition' v (arms:list (Lambda.pattern * exp)) 
-                        (constants:list (pattern * exp))
-                        (pointers:list (pattern * exp)) :=
-     match arms with 
-       | nil => (rev constants, rev pointers, None)
-       | (Lambda.Con_p c nil, e)::rest => partition' v rest ((Con_p c,e)::constants) pointers
-       | (Lambda.Con_p c xs, e)::rest => 
-         partition' v rest constants ((Con_p c,bind_proj v xs 1 e)::pointers)
-       | (Lambda.Var_p x,e)::rest => (rev constants, rev pointers, Some (Let_e (Op_d x v) e))
-     end.
-
-  Definition partition v arms := partition' v arms nil nil.
-  
-  (** Generate a fresh variable -- assumes no user-level variables start with "$". *)
-  Definition freshVar(s:string) : state nat string := LambdaNotation.fresh ("$"%string ++ s).
-  
   (** Simplify a switch that only has one branch. *)
-  Definition SimplSwitch_e (v:op) (arms: list (pattern * exp)) (def:option exp) := 
+  Definition switch_e (v:op) (arms: list (pattern * exp)) (def:option exp) := 
     match arms, def with 
       | (p,e)::nil, None => e
       | _, _ => Switch_e v arms def
     end.
 
-  (** Convert a [Lambda.exp] into a CPS [exp].  The meta-level continuation [k] is used
-      to build the "rest of the expression".  We work in the state monad so we can generate
-      fresh variables.  In general, functions are changed to take an extra argument which
-      is used as the object-level continuation.  We "return" a value [v] by invoking this
-      continuation on [v]. 
+  Section Printing.
+  (** Pretty printing CPS expressions *)
+    Require Import ExtLib.Programming.Show.
+    Require Import Ascii.
+    Import ShowNotation.
+    Local Open Scope string_scope.
+    Local Open Scope show_scope.
 
-      We also must lower Lambda's [Match_e] into CPS's simple Switch.  We are assuming 
-      nullary constructors are represented as "small integers" that can be distinguished 
-      from pointers, and that nary constructors are represented as pointers to tuples that 
-      contain the constructor value in the first field, and the arguments to the 
-      constructors in successive fields.  So for instance, [Cons hd tl] will turn into:
-      [mkTuple_p [Cons, hd, tl]].  
-
-      To do a pattern match on [v], we first test to see if [v] is a pointer.  If not,
-      then we then use a [Switch_e] to dispatch to the appropriate nullary constructor case.
-      If [v] is a pointer, then we extract the construtor tag from the tuple that v
-      references.  We then [Switch_e] on that tag to the appropriate nary constructor
-      case.  The cases then extract the other values from the tuple and bind them to
-      the appropriate pattern variables.  
-  *)
-  Fixpoint cps(e:Lambda.exp)(k:op -> state nat exp) : state nat exp := 
-    match e with 
-      | Lambda.Var_e x => k (Var_o x)
-      | Lambda.Con_e c nil => k (Con_o c)
-      | Lambda.App_e e1 e2 => 
-        cps e1 (fun v1 => 
-          cps e2 (fun v2 => 
-            a <- freshVar "a" ; 
-            e <- k (Var_o a) ; 
-            match match_eta a e with
-              | None => 
-                f <- freshVar "f" ; 
-                ret (Let_e (Fn_d f (a::nil) e) (App_e v1 (v2::(Var_o f)::nil)))
-              | Some c => ret (App_e v1 (v2::c::nil))
-            end))
-      | Lambda.Con_e c es => 
-        (fix cps_es (es:list Lambda.exp) (vs:list op)(k:list op -> state nat exp) : state nat exp := 
-          match es with 
-            | nil => k (rev vs)
-            | e::es => cps e (fun v => cps_es es (v::vs) k)
-          end) es nil
-        (fun vs => 
-          x <- freshVar "x" ; 
-          e <- k (Var_o x) ; 
-          ret (Let_e (Prim_d x MkTuple_p ((Con_o c)::vs)) e))
-      | Lambda.Let_e x e1 e2 => 
-        cps e1 (fun v1 => 
-          e2' <- cps e2 k ; 
-          ret (Let_e (Op_d x v1) e2'))
-      | Lambda.Lam_e x e => 
-        f <- freshVar "f" ; 
-        c <- freshVar "c" ; 
-        e' <- cps e (fun v => ret (App_e (Var_o c) (v::nil))) ; 
-        e0 <- k (Var_o f) ; 
-        ret (Let_e (Fn_d f (x::c::nil) e') e0)
-      | Lambda.Letrec_e fs e => 
-        fs' <- mapM (fun fn => 
-          match fn with 
-            | (f,(x,e)) => 
-              c <- freshVar "c" ; 
-              e' <- cps e (fun v => ret (App_e (Var_o c) (v::nil))) ; 
-              ret (Fn_d f (x::c::nil) e')
-          end) fs ; 
-        e0 <- cps e k ; 
-        ret (Let_e (Rec_d fs') e0)
-      | Lambda.Match_e e arms => 
-        cps e (fun v => 
-          x <- freshVar "x" ; 
-          e0 <- k (Var_o x) ; 
-          c <- freshVar "c" ; 
-          cont <- match match_eta x e0 with
-                    | None => ret (Var_o c)
-                    | Some v' => ret v'
-                  end ;
-          arms' <- mapM (fun p_e => e' <- cps (snd (p_e)) (fun v => ret (App_e cont (v::nil))) ;
-            ret (fst p_e, e')) arms ; 
-          is_ptr <- freshVar "isptr" ; 
-          tag <- freshVar "tag" ; 
-          m <- match partition v arms' with 
-                 | (constant_arms, pointer_arms, def) => 
-                   ret (Let_e (Prim_d is_ptr Ptr_p (v::nil))
-                     (Switch_e (Var_o is_ptr)
-                       ((Con_p "false"%string, SimplSwitch_e v constant_arms def)::
-                         (Con_p "true"%string, 
-                           (Let_e (Prim_d tag Proj_p ((Int_o 0)::v::nil))
-                             (SimplSwitch_e (Var_o tag) pointer_arms def)))::nil) None))
-               end ; 
-          match match_eta x e0 with 
-            | None => ret (Let_e (Fn_d c (x::nil) e0) m)
-            | Some _ => ret m
-          end
-          )
-    end.
-
-  Definition CPS(e:Lambda.exp) : exp := 
-    fst (runState (cps e (fun x => ret (Halt_e x))) 0).
-
-  Section CPSEVAL.
-    (** Because this version of CPS supports recursive records, as well as recursive
-        functions, I've chosen to use an allocation-style semantics here, where large
-        values, such as tuples and closures, are allocated on a heap.  Then, to build
-        circular values, such as recursive closures or recursive tuples, we first 
-        allocate space for them, then initialize them with back-patching. *)
-
-    (** Small values *)
-    Inductive value : Type := 
-    | Con_v : constructor -> value
-    | Int_v : Z -> value
-    | Ptr_v : nat -> value.
-
-    (** Allocated values *)
-    Inductive heap_value : Type := 
-    | Tuple_v : list value -> heap_value
-    | Closure_v : env_t value -> list var -> exp -> heap_value.
-
-    (** We'll just naively implement heaps as lists of heap values *)
-    Definition heap := list heap_value.
-
-    (** We'll be working in a combination of the state and option monads, so
-        I've written various environment and other functions tailored to that
-        monad. *)
-    Fixpoint lookup {A} (env:env_t A) (x:var) : optionT (state heap) A := 
-      match env with 
-        | nil => zero
-        | (y,v)::rest => if eq_dec y x then ret v else lookup rest x 
+    Fixpoint spaces (n:nat) : showM :=
+      match n with
+        | 0 => empty
+        | S n => " "%char << spaces n
       end.
 
-    Definition extend {A} (env:env_t A) (x:var) (v:A) : env_t A := (x,v)::env.
+    Global Instance Show_positive : Show positive :=
+      { show p := show (Pos.to_nat p) }.
 
-    Fixpoint extends {A}(env:env_t A) (xs:list var) (vs:list A) : optionT (state heap) (env_t A) := 
-      match xs, vs with 
-        | nil, nil => ret env
-        | x::xs, v::vs => extends (extend env x v) xs vs
-        | _, _ => zero
+    Global Instance Show_Z : Show Z :=
+      { show x :=
+        match x with 
+          | Z0 => "0"%char
+          | Zpos p => show p
+          | Zneg p => "-"%char << show p
+        end }.
+    Global Instance Show_op : Show op :=
+      { show o :=
+        match o with 
+          | Var_o x => show x
+          | Con_o c => "Con(" << show c << ")"
+          | Int_o i => show i
+        end }.
+    Global Instance Show_pat : Show pattern :=
+      { show p :=
+        match p with 
+          | Int_p i => show i
+          | Con_p c => show c
+        end }.
+    Global Instance Show_primop : Show primop :=
+      { show p := 
+        match p with 
+          | Eq_p => "eq?"
+          | Neq_p => "neq?"
+          | Lt_p => "lt?"
+          | Lte_p => "lte?"
+          | Ptr_p => "ptr?"
+          | Plus_p => "+"
+          | Minus_p => "-"
+          | Times_p => "*"
+          | Proj_p => "#"
+          | MkTuple_p => "mkTuple"
+        end }.
+
+    Fixpoint sepBy (sep : showM) (ls : list showM) : showM :=
+      match ls with
+        | nil => empty
+        | l :: nil => l
+        | l :: ls => l << sep << sepBy sep ls
       end.
+    Require Import ExtLib.Data.Char.
+    
+    Fixpoint emitexp (e:exp) : showM :=
+      match e with 
+        | App_e v vs => show v << "(" << sepBy " " (map show vs) << ")"
+        | Let_e d e =>
+          "let " << indent "  " (emitdecl false d) << "in " << indent "  " (emitexp e)
+        | Switch_e v arms def => 
+          "switch " << empty (*show v*) << " with" << empty (*
+          indent "  " (
+            iterM (fun (p: pattern * exp) => 
+              chr_newline << "| " << show (fst p) << " => " << emitexp (snd p)) arms
+            << match def with 
+                 | None => empty
+                 | Some e => chr_newline << "| _ => " << emitexp e
+               end) *)
+          << chr_newline << "end"
+        | Halt_e o => "HALT " << show o
+      end
+    with emitdecl (inrec:bool) (d:decl) : showM := 
+      let emit_sep : showM := if inrec then " and" else " in" in 
+        match d with 
+          | Op_d x v => 
+            show x << " = " << show v << emit_sep 
+          | Prim_d x p vs => 
+            show x << " = " << show p << "(" << sepBy " " (map show vs) << ")" << emit_sep 
+          | Fn_d f xs e => 
+            show f << "(" << sepBy (", " : showM) (map show xs) << ") = " << indent "  " (emitexp e) << emit_sep 
+          | Rec_d ds => 
+          "rec "<< sepBy chr_newline (map (emitdecl true) ds)
+        end.
 
-    Definition eval_op (env:env_t value) (v:op) : optionT (state heap) value := 
-      match v with 
-        | Con_o c => ret (Con_v c)
-        | Int_o i => ret (Int_v i)
-        | Var_o x => lookup env x
-      end.
+    Global Instance Show_exp : Show exp := emitexp.
+    Global Instance Show_decl : Show decl := emitdecl false.
 
-    (** Find the appropriate switch arm for a given small value. *)
-    Fixpoint find_arm (v:value) (arms : list (pattern * exp)) (def:option exp) : optionT (state heap) exp := 
-      match v,arms with 
-        | _,nil => match def with | None => zero | Some e => ret e end
-        | Con_v c, ((Con_p c',e)::rest) => if eq_dec c c' then ret e else find_arm v rest def
-        | Int_v i, ((Int_p i',e)::rest) => if eq_dec i i' then ret e else find_arm v rest def
-        | _,(_::rest) => find_arm v rest def
-      end.
-
-    (** Allocate a heap value and return its address as a pointer *)
-    Definition malloc(v:heap_value) : optionT (state heap) value := 
-      h <- get ;
-      put (h ++ (v::nil)) ;; 
-      ret (Ptr_v (List.length h)).
-
-    (** Lookup the pointer [n] in the heap. *)
-    Definition heap_lookup (n:nat) : optionT (state heap) heap_value := 
-      h <- get ; 
-      match nth_error h n with 
-        | None => zero
-        | Some v => ret v
-      end.
-
-    Fixpoint heap_upd (n:nat) (h:heap) (v:heap_value) : option heap := 
-      match n, h with 
-        | 0, _::tail => ret (v::tail)
-        | S n, head::tail => t <- (heap_upd n tail v) ; ret (head::t)
-        | _, _ => None
-      end.
-
-    (** Update the heap value at location [n] to be the value [v]. *)
-    Definition heap_set (n:nat) (v:heap_value) : optionT (state heap) unit := 
-      h <- get ; 
-      match heap_upd n h v with 
-        | None => zero
-        | Some h' => put h'
-      end.
-
-    (** Evaluate the primops given closed values *)      
-    Definition eval_primop (p:primop) (vs: list value) : optionT (state heap) value := 
-      match p, vs with 
-        | Eq_p, (Int_v i)::(Int_v j)::nil => ret (if eq_dec i j then (Con_v "true") else (Con_v "false"))
-        | Eq_p, (Con_v i)::(Con_v j)::nil => ret (if eq_dec i j then (Con_v "true") else (Con_v "false"))
-        | Neq_p, (Int_v i)::(Int_v j)::nil => ret (if eq_dec i j then (Con_v "false") else (Con_v "true"))
-        | Neq_p, (Con_v i)::(Con_v j)::nil => ret (if eq_dec i j then (Con_v "false") else (Con_v "true"))
-        | Lt_p, (Int_v i)::(Int_v j)::nil => ret (if Z.ltb i j then (Con_v "true") else (Con_v "false"))
-        | Lte_p, (Int_v i)::(Int_v j)::nil => ret (if orb (Z.ltb i j) (eq_dec i j) 
-                                                   then (Con_v "true") else (Con_v "false"))
-        | Ptr_p, ((Int_v _)::nil) => ret (Con_v "false")
-        | Ptr_p, ((Con_v _)::nil) => ret (Con_v "false")
-        | Ptr_p, ((Ptr_v _)::nil) => ret (Con_v "true")
-        | Plus_p, ((Int_v i)::(Int_v j)::nil) => ret (Int_v (i+j))
-        | Minus_p, ((Int_v i)::(Int_v j)::nil) => ret (Int_v (i-j))
-        | Times_p, ((Int_v i)::(Int_v j)::nil) => ret (Int_v (i*j))
-          (** Note allocation here *)
-        | MkTuple_p, vs => malloc (Tuple_v vs)
-        | Proj_p, ((Int_v i)::(Ptr_v n)::nil) => 
-          (** Lookup the pointer in the heap to get a heap value [v] *)
-          v <- heap_lookup n ; 
-          match v with 
-            (** Check that [v] is a tuple *)
-            | Tuple_v vs => 
-              match nth_error vs (Z.abs_nat i) with 
-                | None => zero
-                | Some v => ret v
-              end
-            | _ => zero
-          end
-        | _, _ => zero
-      end%string.
-
-    (** Used for initializing variables to some pointer value to a dummy
-       heap value in a circular set of definitions. *)
-    Definition malloc_dummy (d:decl) : optionT (state heap) (var * value) := 
-      match d with 
-        | Fn_d f _ _ => v <- malloc (Tuple_v nil) ; ret (f,v)
-        | Prim_d x MkTuple_p _ => v <- malloc (Tuple_v nil) ; ret (x,v)
-        | _ => zero
-      end.
-
-    (** Assuming we've already bound the declared variable in [d] to a pointer
-        value [p], we now actually build the appropriate value under this 
-        extended environment.  Then we set [p] to point to the new value.
-        So for instance, if we have:
-
-        let rec x = MkTuple [x;x]
-
-        then we first allocate a dummy empty tuple at location [p] and update
-        the environment so [x] maps to [p].  Then we actually build the 
-        tuple, evaluating the components to closed values.  In this case,
-        we'd get a [Tuple_v [p;p]].  Finally, we set [p] to point to this
-        heap value.  So in the end, we have an environment that maps [x] to
-        [p], and a heap that maps [p] to [Tuple_v [p;p]].  
-
-        Note that we only support recursion on functions and tuples and not,
-        in general, on arbitrary declarations.  This ensures that we don't
-        end up evaluating something that eliminates a pointer (e.g., projection,
-        or function call) when we haven't completed initializing the expression.
-
-        Another advantage of making this all explicit is that it's quite
-        close to what we'll do at the machine level.
-     *)
-    Definition initialize_decl(env:env_t value) (d: decl) : optionT (state heap) unit :=
-      match d with 
-        | Fn_d f xs e => 
-          v <- lookup env f ; 
-          match v with 
-            | Ptr_v n => heap_set n (Closure_v env xs e)
-            | _ => zero
-          end
-        | Prim_d x MkTuple_p vs => 
-          vs' <- mapM (eval_op env) vs ; 
-          v <- lookup env x ; 
-          match v with 
-            | Ptr_v n => heap_set n (Tuple_v vs')
-            | _ => zero
-          end
-        | _ => zero
-      end.
-
-    Fixpoint eval_decl (env:env_t value) (d:decl) : optionT (state heap) (env_t value) := 
-      match d with 
-        | Op_d x v => v' <- eval_op env v ; ret (extend env x v')
-        | Fn_d f xs e => p <- malloc (Closure_v env xs e) ; ret (extend env f p)
-        | Prim_d x p vs => vs' <- mapM (eval_op env) vs ; v <- eval_primop p vs' ; ret (extend env x v)
-        | Rec_d ds => 
-          env' <- mapM malloc_dummy ds ; 
-          _ <- mapM (initialize_decl (env' ++ env)) ds ; 
-          ret (env' ++ env)
-      end.
-
-    Fixpoint eval_exp (n:nat)(env:env_t value) (e:exp) : optionT (state heap) (list value) := 
-      match n with 
-        | 0 => zero
-        | S n => 
-          match e with 
-            | App_e v vs => 
-              v' <- eval_op env v ; vs' <- mapM (eval_op env) vs ; 
-              match v' with 
-                | Ptr_v z => 
-                  hv <- heap_lookup z ; 
-                  match hv with 
-                    | Closure_v env xs e => env' <- extends env xs vs' ; eval_exp n env' e
-                    | _ => zero
-                  end
-                | _ => zero
-              end
-            | Let_e d e => env' <- eval_decl env d ; eval_exp n env' e
-            | Switch_e v arms def => 
-              v' <- eval_op env v ; e <- find_arm v' arms def ; eval_exp n env e
-            | Halt_e o => x <- eval_op env o ;; ret (x::nil)
-          end 
-      end.
-
-    Definition run {A} (c : optionT (state heap) A) (h:heap) : option A * heap := 
-      runState (unOptionT c) h.
-
-    Definition eval (n:nat) (e:exp) : option (list value) * heap := run (eval_exp n nil e) nil.
-
-    (*
-    Section TEST_EVAL.
-      Import LambdaNotation. 
-      Local Open Scope string_scope.
-
-      Eval compute in exp2string (CPS (gen ((\x => x) @ Z_c))).
-      Eval compute in eval 100 (CPS (gen ((\x => x) @ Z_c))).
-
-      Eval compute in exp2string (CPS (gen e1)).
-      Eval compute in eval 100 (CPS (gen e1)).
-
-      Eval compute in exp2string (CPS (gen e2)).
-      Eval compute in eval 100 (CPS (gen e2)).
-
-      Eval compute in exp2string (CPS (gen e3)).
-      Eval compute in eval 100 (CPS (gen e3)).
-
-      Eval compute in exp2string (CPS (gen e4)).
-      Eval compute in eval 100 (CPS (gen e4)).  (** Evalutes to None in 100 steps because it diverges *)
-
-      Eval compute in exp2string (CPS (gen e5)).
-      Eval compute in eval 100 (CPS (gen e5)).  
-
-      Eval compute in exp2string (CPS (gen e6)).
-      Eval compute in eval 100 (CPS (gen e6)).
-
-      Eval compute in exp2string (CPS (gen e7)).
-      Eval compute in eval 100 (CPS (gen e7)).
-
-      Eval compute in exp2string (CPS (gen e8)).
-      Eval compute in eval 100 (CPS (gen e8)).
-    End TEST_EVAL.
-    *)
-  End CPSEVAL.
+    Definition exp2string (e:exp) : string := 
+      @runShow (string -> string) _ (show e) "".
+    
+  End Printing.
 
 End CPS.
+
+Export Env.
