src/Env.v
@@ -1,5 +1,11 @@
-Require Import List.
-Require Import ExtLib.FMaps.FMaps.
+Require Import List BinPos String.
+Require Import ExtLib.Structures.Maps.
+Require Import ExtLib.Core.RelDec.
+Require Import ExtLib.Core.CmpDec.
+Require Import ExtLib.Core.PosDecidables.
+Require Import ExtLib.Data.Strings.
+Require Import ExtLib.Programming.Show.
+Require Import ExtLib.Tactics.Consider.
 
 Set Implicit Arguments.
 Set Strict Implicit.
@@ -7,7 +13,7 @@ Set Strict Implicit.
 Section with_map.
   Variable map : Type -> Type.
   Variable K : Type.
-  Context {Map_map : Map K map}.
+  Context {Map_map : DMap K map}.
 
   Fixpoint add_all {A} (m : map A) (xs:list K) (vs:list A) : map A :=
     match xs, vs with
@@ -15,3 +21,57 @@ Section with_map.
       | _, _ => m
     end.
 End with_map.
+
+Inductive var := 
+| Anon_v : positive -> var
+| Named_v : string -> option positive -> var.
+
+Definition mkVar (v : option string) (n : positive) : var :=
+  match v with
+    | None => Anon_v n
+    | Some s => Named_v s (Some n)
+  end.
+
+Definition wrapVar (v : string) : var :=
+  Named_v v None.
+
+Global Instance RelDec_var_eq : RelDec (@eq var) :=
+{ rel_dec x y :=
+    match x , y with
+      | Anon_v x , Anon_v y => eq_dec x y
+      | Named_v x xi , Named_v y yi =>
+        if eq_dec x y then eq_dec xi yi else false
+      | _ , _ => false
+    end }.
+
+Global Instance RelDec_Correct_var_eq : RelDec_Correct RelDec_var_eq.
+Proof.
+  Opaque RelDec_peq.
+  constructor.  destruct x; destruct y; intros; simpl in *; intuition; try congruence.
+  consider (eq_dec p p0); intros; subst; auto.
+  inversion H; clear H; subst.
+  consider (eq_dec p0 p0); auto.
+  consider (string_dec s s0); intros; subst.
+  destruct o; destruct o0; try congruence.
+  consider (eq_dec p p0); intros; subst; auto.
+  inversion H; clear H; subst.
+  consider (string_dec s0 s0); try congruence; intros.
+  destruct o0; auto. consider (eq_dec p p); auto.
+Qed.
+
+Global Instance CmpDec_positive : CmpDec (@eq positive) Pos.lt :=
+{ cmp_dec := Pos.compare }.
+
+Section hiding_notation.
+  Import ShowNotation.
+  Require Import Ascii.
+  Local Open Scope show.
+
+  Global Instance Show_var : Show var :=
+    fun x =>
+      match x with
+        | Anon_v p => "$"%char << show p
+        | Named_v n None => n
+        | Named_v n (Some p) => n << "_"%char << show p
+      end.
+End hiding_notation.
