src/LLVM.v
@@ -1,10 +1,11 @@
 Require Import Lambda Cps.
 Require Import ZArith String List Bool.
-Require Import ExtLib.Monad.Monad.
-Require Import ExtLib.Monad.OptionMonad ExtLib.Monad.StateMonad.
-Require Import ExtLib.Monad.Folds.
+Require Import ExtLib.Structures.Monads.
+Require Import ExtLib.Data.Monads.OptionMonad.
+Require Import ExtLib.Data.Monads.StateMonad.
+Require Import ExtLib.Structures.Folds.
 Require Import ExtLib.Data.Strings.
-Require Import ExtLib.Decidables.Decidable.
+Require Import ExtLib.Core.RelDec.
 Require Import ExtLib.Tactics.Consider.
 
 Set Implicit Arguments.
@@ -24,11 +25,9 @@ Module LLVM.
   Import MonadNotation String.
   Local Open Scope string_scope.
   Local Open Scope monad_scope.
-  Definition var := Lambda.var.
   Definition constructor := Lambda.constructor.
+  Definition var := string.
   Definition env_t := Lambda.env_t.
-  Definition string_of_nat := LambdaNotation.nat2string.
-  Definition string_of_Z := CPS.z2string.
   Definition label := string.
 
   Inductive cconv : Type := 
@@ -38,72 +37,23 @@ Module LLVM.
   Definition quoted (s:string) := 
     String double_quote (s ++ (String double_quote EmptyString)).
 
-  Definition string_of_cconv (c:cconv) : string := 
-    (* quoted *)
-    match c with 
-      | X86_fastcallcc => "x86_fastcallcc" 
-      | C_cc => "ccc" | Fast_cc => "fastcc" | Cold_cc => "coldcc" | CC10_cc => "cc 10"
-      | Num_cc n => "cc " ++ (string_of_nat n)
-    end.
-
   Inductive linkage : Type := 
   | Private | Linker_private | Linker_private_weak | Linker_private_weak_def_auto 
   | Internal | Available_externally | Linkonce | Weak | Common | Appending | Extern_weak
   | Linkonce_odr | Weak_odr | External | Dllimport | Dllexport. 
-
-  Definition string_of_linkage (l:linkage) : string := 
-    match l with 
-      | Private => "private"
-      | Linker_private => "linker_private"
-      | Linker_private_weak => "linker_private_weak"
-      | Linker_private_weak_def_auto => "linker_private_weak_def_auto"
-      | Internal => "internal"
-      | Available_externally => "available_externally"
-      | Linkonce => "linkonce"
-      | Weak => "weak"
-      | Common => "common"
-      | Appending => "appending"
-      | Extern_weak => "extern_weak"
-      | Linkonce_odr => "linkonce_odr"
-      | Weak_odr => "weak_odr"
-      | External => "external"
-      | Dllimport => "dllimport"
-      | Dllexport => "dllexport"
-    end.
       
   Inductive visibility : Type := | Default_v | Hidden_v | Protected_v.
-
-  Definition string_of_visibility (v:visibility) : string := 
-    quoted 
-    match v with 
-      | Default_v => "default" | Hidden_v => "hidden" | Protected_v => "protected"
-    end.
 
   Inductive param_attr : Type := 
   | Zeroext_pattr | Signext_pattr | Inreg_pattr | Byval_pattr | Sret_pattr | Noalias_pattr
   | Nocapture_pattr | Nest_pattr.
 
-  Definition string_of_param_attr (p:param_attr) : string := 
-    match p with 
-      | Zeroext_pattr => "zeroext" | Signext_pattr => "signext" | Inreg_pattr => "inreg" 
-      | Byval_pattr => "byval" | Sret_pattr => "sret" | Noalias_pattr => "noalias"
-      | Nocapture_pattr => "nocapture" | Nest_pattr => "nest"
-    end.
 
   Inductive fn_attr : Type := 
   | Address_safety | Align_stack : nat -> fn_attr | Alwaysinline | Nonlazybind | Inlinehint
   | Naked | Noimplicitfloat | Noinline | Noredzone | Noreturn | Nounwind
   | Optsize | Readnone | Readonly | Returns_twice | Ssp | Sspreq | Uwtable.
 
-  Definition string_of_fn_attr(f: fn_attr) : string := 
-    match f with 
-      | Address_safety => "address_safety" | Align_stack n => "alignstack(" ++ (string_of_nat n) ++ ")" 
-      | Alwaysinline => "alwaysinline" | Nonlazybind => "nonlazybind" | Inlinehint => "inlinehint"
-      | Naked => "naked" | Noimplicitfloat => "noimplicitfloat" | Noinline => "noinline" 
-      | Noredzone => "noredzone" | Noreturn => "noreturn" | Nounwind => "nounwind"
-      | Optsize => "optsize" | Readnone => "readnone" | Readonly => "readonly" 
-      | Returns_twice => "returns_twice" | Ssp => "ssp" | Sspreq => "sspreq" | Uwtable => "uwtable"
-    end.
 
   Inductive type : Type := 
   | I_t : nat -> type
@@ -112,39 +62,10 @@ Module LLVM.
   | Array_t : list nat -> type -> type
   | Fn_t : forall (returntype: type) (arg_types : list type) (vararg : bool), type
   | Struct_t : forall (packed:bool) (elts : list type), type
-  | Named_t : var -> type
+  | Named_t : string -> type
   | Opaque_t : type
   | Pointer_t : forall (addrspace:nat), type -> type
   | Vector_t : nat -> type -> type.
-
-  Fixpoint sep (s:string) (ss:list string) : string := 
-    match ss with 
-      | nil => ""
-      | h::nil => h
-      | h::t => h ++ s ++ (sep s t)
-    end.
-
-  Fixpoint string_of_type (t:type) : string := 
-    match t with 
-      | I_t n => "i" ++ (string_of_nat n)
-      | Half_t => "half" | Float_t => "float" | Double_t => "double" | X86_fp80_t => "x86_fp80"
-      | Fp128_t => "fp128" | Ppc_fp128_t => "ppc_fp128" | Void_t => "void" | Label_t => "label"
-      | X86mmx_t => "x86mmx" | Metadata_t => "metadata"
-      | Array_t ns t => 
-        List.fold_right (fun (i:nat) (t:string) => 
-                         "[" ++ (string_of_nat i) ++ " x " ++ t ++ "]") (string_of_type t) ns
-      | Fn_t t ts vararg => 
-        (string_of_type t) ++ "(" ++ (sep ", " (List.map string_of_type ts)) ++ 
-        (if vararg then ",...)" else ")")
-      | Struct_t packed elts => 
-        let s := "{" ++ (sep ", " (List.map string_of_type elts)) ++ "}" in 
-          if packed then "<" ++ s ++ ">" else s
-      | Named_t x => x
-      | Opaque_t => "opaque"
-      | Pointer_t 0 t => (string_of_type t) ++ " *"
-      | Pointer_t n t => (string_of_type t) ++ "addrspace(" ++ (string_of_nat n) ++ ") *"
-      | Vector_t n t => "<" ++ (string_of_nat n) ++ " x " ++ (string_of_type t) ++ ">"
-    end.
 
   Inductive constant : Type := 
   | True_c
@@ -161,19 +82,6 @@ Module LLVM.
   | Metadata_c : list constant -> constant
   | Metastring_c : string -> constant.
 
-  Fixpoint string_of_constant (c:constant) : string := 
-    match c with 
-      | True_c => "true" | False_c => "false" 
-      | Int_c i => string_of_Z i
-      | Float_c s => s | Null_c =>  "null" | Global_c v => v 
-      | Undef_c => "undef" | Zero_c => "zeroinitializer"
-      | Struct_c cs => "{" ++ (sep ", " (List.map string_of_constant cs)) ++ "}"
-      | Array_c cs => "[" ++ (sep ", " (List.map string_of_constant cs)) ++ "]"
-      | Vector_c cs => "<" ++ (sep ", " (List.map string_of_constant cs)) ++ ">"
-      | Metastring_c s => "!" ++ (quoted s)
-      | Metadata_c cs => "!{" ++ (sep ", " (List.map string_of_constant cs)) ++ "}"
-    end.
-
   Inductive value : Type := 
   | Local : var -> value
   | Global : var -> value
@@ -181,35 +89,12 @@ Module LLVM.
   | AnonGlobal : nat -> value
   | Constant : constant -> value.
 
-  Definition string_of_value(v:value) : string := 
-    match v with 
-      | Local x => "%" ++ x
-      | Global x => "@" ++ x
-      | AnonLocal n => "%" ++ (string_of_nat n)
-      | AnonGlobal n => "@" ++ (string_of_nat n)
-      | Constant c => string_of_constant c
-    end.
-
   Inductive cond : Type := 
   | Eq | Ne | Ugt | Uge | Ult | Ule | Sgt | Sge | Slt | Sle.
-
-  Definition string_of_cond(c:cond) : string := 
-    match c with 
-      | Eq => "eq" | Ne => "ne" | Ugt => "ugt" | Uge => "uge" | Ult => "ult" | Ule => "ule" 
-      | Sgt => "sgt" | Sge => "sge" | Slt => "slt" | Sle => "sle"
-    end.
 
   Inductive fcond : Type := 
   | False_fc | Oeq_fc | Ogt_fc | Oge_fc | Olt_fc | Ole_fc | One_fc | Ord_fc | Ueq_fc
   | Ugt_fc | Uge_fc | Ult_fc | Ule_fc | Une_fc | Uno_fc | True_fc.
-
-  Definition string_of_fcond(f:fcond) : string := 
-    match f with 
-      | False_fc => "false" | Oeq_fc => "oeq" | Ogt_fc => "ogt" | Oge_fc => "oge" | Olt_fc => "olt"
-      | Ole_fc => "ole" | One_fc => "one" | Ord_fc => "ord" | Ueq_fc => "ueq" | Ugt_fc => "ugt"
-      | Uge_fc => "uge" | Ult_fc => "ult" | Ule_fc => "ule" | Une_fc => "une" | Uno_fc => "uno"
-      | True_fc => "true"
-    end.
 
   Inductive exp : Type := 
   | Add_e : forall (nuw:bool) (nsw:bool) (ty:type) (op1:value) (op2:value), exp
@@ -258,6 +143,277 @@ Module LLVM.
                     (fn_attrs: list fn_attr), exp.
 
   Definition flag(b:bool)(s:string) : string := if b then s else "".
+  
+  Inductive instr : Type := 
+  | Comment_i : string -> instr
+  | Ret_i : option (type * value) -> instr
+  | Br_cond_i : value -> label -> label -> instr
+  | Br_uncond_i : label -> instr
+  | Switch_i : type -> value -> label -> list (type * Z * label) -> instr
+  | Resume_i : type -> value -> instr
+  | Unreachable_i : instr
+  | Assign_i : (option value) -> exp -> instr
+  | Store_i : forall (atomic:bool) (volatile:bool) (ty:type) (v:value) (ptrty:type) (pointer:value) 
+                     (align:option nat) (nontemporal:option nat) (singlethread:bool), instr.
+
+  Record fn_header : Type := {
+    linkage_fh : option linkage ; 
+    visibility_fh : option visibility ; 
+    cconv_fh : option cconv ; 
+    unnamed_addr_fh : bool ; 
+    return_type_fh : type ; 
+    return_type_attrs_fh : list param_attr ; 
+    name_fh : var ; 
+    args_fh : list (type * var * list (param_attr)) ; 
+    attrs_fh : list fn_attr ; 
+    section_fh : option string ; 
+    align_fh : option nat ; 
+    gc_fh : option string
+  }.
+
+  Definition block := ((option label) * (list instr))%type.
+    
+  Inductive topdecl : Type := 
+  | Global_d : forall (x:var) (addrspace:option nat) (l:option linkage) (unnamed_addr:bool) (const:bool) 
+                      (t:type) (c:constant) (section:option string) (align:option nat), topdecl
+  | Define_d : fn_header -> list block -> topdecl
+  | Declare_d : fn_header -> topdecl
+  | Alias_d : forall (x:var) (l:option linkage) (v:option visibility) (t:type) (e:exp), topdecl
+  | Metadata_d : forall (x:var), list constant -> topdecl.
+
+  Definition module := list topdecl.
+
+  Section Printing.
+    Require Import ExtLib.Programming.Show.
+    Import ShowNotation.
+    (** TODO **)
+    Global Instance Show_module : Show module := fun _ => "<TODO>".
+
+  End Printing.
+End LLVM.
+
+(*
+  Definition emit_option {A} (f:A -> ST unit) (x:option A) : ST unit := 
+    match x with 
+      | None => ret tt
+      | Some v => f v 
+    end.
+  Definition emit_option_s {A} (f:A -> ST unit) (x:option A) : ST unit := 
+    match x with 
+      | None => ret tt
+      | Some v => f v ;; emit " "
+    end.
+
+  Definition emit_instr (i:instr) : state (list string) unit := 
+    spaces 4 ;; emit (string_of_instr i) ;; newline.
+
+
+
+  Definition emit_block (b:block) : state (list string) unit := 
+    emit_option (fun l => spaces 2 ;; emit l ;; emit ":" ;; newline) (fst b) ;; 
+    iter emit_instr (snd b).
+
+  Definition pipe {A B C} (f:B -> C) (g:A -> B) : A -> C := 
+    fun x => f (g x).
+
+  Infix "$" := pipe (at level 70, right associativity).
+
+
+  Definition emit_fn_header (drop_vars:bool) (fh:fn_header) : state (list string) unit := 
+    emit_option_s (emit $ string_of_linkage) (linkage_fh fh) ;; 
+    emit_option_s (emit $ string_of_visibility) (visibility_fh fh) ;; 
+    emit_option_s (emit $ string_of_cconv) (cconv_fh fh) ;;
+    (if (unnamed_addr_fh fh) then emit "unnamed_addr " else ret tt) ;; 
+    emit (string_of_type (return_type_fh fh)) ;; emit " " ;;
+    iter (fun x => emit (string_of_param_attr x) ;; emit " ") (return_type_attrs_fh fh) ;;
+    emit "@" ;; emit (name_fh fh) ;; emit "(" ;; 
+    sepby (fun p => match p with (t,x,attrs) => 
+                     emit (string_of_type t) ;; 
+                     (if drop_vars then ret tt else emit " %"%string ;; emit x) ;;
+                     iter (fun x => emit (string_of_param_attr x) ;; emit " ") attrs
+                   end) (emit ", ") (args_fh fh) ;;
+    emit ") " ;;
+    iter (fun x => emit (string_of_fn_attr x) ;; emit " ") (attrs_fh fh) ;;
+    emit_option_s (fun s => emit ", section " ;; emit (quoted s) ;; emit " ") (section_fh fh) ;;
+    emit_option_s (fun n => emit ", align " ;; emit (string_of_nat n) ;; emit " ") (align_fh fh) ;;
+    emit_option_s (fun s => emit "gc " ;; emit (quoted s) ;; emit " ") (gc_fh fh).
+
+
+
+  Definition emit_topdecl (t:topdecl) : ST unit := 
+    match t with 
+      | Global_d x a l u c t v s al => 
+        emit x ;; emit " = " ;;
+        emit_option_s (fun n => emit "addrspace(" ;; emit (string_of_nat n) ;; emit ")") a ;;
+        emit_option_s (emit $ string_of_linkage) l ;;
+        (if u then emit "unnamed_addr " else ret tt) ;;
+        (if c then emit "constant " else ret tt) ;;
+        emit (string_of_type t) ;; emit " " ;; 
+        emit (string_of_constant v) ;; emit " " ;;
+        emit_option_s (fun s => emit ", section " ;; emit (quoted s) ;; emit " ") s ;;
+        emit_option_s (fun n => emit ", align " ;; emit (string_of_nat n) ;; emit " ") al ;;
+        newline 
+      | Define_d fh bs => emit "define " ;;
+        emit_fn_header false fh ;; emit " {" ;; newline ;; iter emit_block bs ;; emit "}" ;; newline
+      | Declare_d fh => emit "declare " ;; emit_fn_header true fh ;; newline
+      | Alias_d x l v t e => 
+        emit x ;; emit " = alias " ;; 
+        emit_option_s (emit $ string_of_linkage) l ;;
+        emit_option_s (emit $ string_of_visibility) v ;;
+        emit (string_of_type t) ;; emit " " ;; 
+        emit (string_of_exp e) ;; newline
+      | Metadata_d x cs => 
+        emit x ;; emit " = metadata !{" ;; emit (sep ", " (List.map string_of_constant cs)) ;; 
+        emit "}" ;; newline
+    end.
+
+
+  Definition emit_module (m:module) : ST unit := iter emit_topdecl m.
+
+  Definition runST (c:ST unit) := 
+    List.fold_left (fun x y => y ++ x) (snd (runState c nil)).
+
+  Definition string_of_module := runST $ emit_module.
+  Definition string_of_topdecl := runST $ emit_topdecl.
+  Definition string_of_fn_header b := runST $ (emit_fn_header b).
+
+  (* 
+  Definition test_block : block := (None, Comment_i "Here is a comment." :: Ret_i None :: nil).
+  Definition test : topdecl :=
+    Define_d
+    {|
+      linkage_fh := None;
+      visibility_fh := None;
+      cconv_fh := None;
+      unnamed_addr_fh := false;
+      return_type_fh := I_t 3;
+      return_type_attrs_fh := nil;
+      name_fh := "test";
+      args_fh := nil;
+      attrs_fh := nil;
+      section_fh := None;
+      align_fh := None;
+      gc_fh := None |} 
+    (test_block :: nil).
+
+  Eval compute in (string_of_topdecl test "").
+  *)
+
+
+End LLVM.
+
+
+
+  Definition string_of_cconv (c:cconv) : string := 
+    (* quoted *)
+    match c with 
+      | X86_fastcallcc => "x86_fastcallcc" 
+      | C_cc => "ccc" | Fast_cc => "fastcc" | Cold_cc => "coldcc" | CC10_cc => "cc 10"
+      | Num_cc n => "cc " ++ (string_of_nat n)
+    end.
+
+  Definition string_of_linkage (l:linkage) : string := 
+    match l with 
+      | Private => "private"
+      | Linker_private => "linker_private"
+      | Linker_private_weak => "linker_private_weak"
+      | Linker_private_weak_def_auto => "linker_private_weak_def_auto"
+      | Internal => "internal"
+      | Available_externally => "available_externally"
+      | Linkonce => "linkonce"
+      | Weak => "weak"
+      | Common => "common"
+      | Appending => "appending"
+      | Extern_weak => "extern_weak"
+      | Linkonce_odr => "linkonce_odr"
+      | Weak_odr => "weak_odr"
+      | External => "external"
+      | Dllimport => "dllimport"
+      | Dllexport => "dllexport"
+    end.
+
+  Definition string_of_param_attr (p:param_attr) : string := 
+    match p with 
+      | Zeroext_pattr => "zeroext" | Signext_pattr => "signext" | Inreg_pattr => "inreg" 
+      | Byval_pattr => "byval" | Sret_pattr => "sret" | Noalias_pattr => "noalias"
+      | Nocapture_pattr => "nocapture" | Nest_pattr => "nest"
+    end.
+
+
+  Definition string_of_visibility (v:visibility) : string := 
+    quoted 
+    match v with 
+      | Default_v => "default" | Hidden_v => "hidden" | Protected_v => "protected"
+    end.
+
+  Definition string_of_fn_attr(f: fn_attr) : string := 
+    match f with 
+      | Address_safety => "address_safety" | Align_stack n => "alignstack(" ++ (string_of_nat n) ++ ")" 
+      | Alwaysinline => "alwaysinline" | Nonlazybind => "nonlazybind" | Inlinehint => "inlinehint"
+      | Naked => "naked" | Noimplicitfloat => "noimplicitfloat" | Noinline => "noinline" 
+      | Noredzone => "noredzone" | Noreturn => "noreturn" | Nounwind => "nounwind"
+      | Optsize => "optsize" | Readnone => "readnone" | Readonly => "readonly" 
+      | Returns_twice => "returns_twice" | Ssp => "ssp" | Sspreq => "sspreq" | Uwtable => "uwtable"
+    end.
+
+
+  Fixpoint string_of_type (t:type) : string := 
+    match t with 
+      | I_t n => "i" ++ (string_of_nat n)
+      | Half_t => "half" | Float_t => "float" | Double_t => "double" | X86_fp80_t => "x86_fp80"
+      | Fp128_t => "fp128" | Ppc_fp128_t => "ppc_fp128" | Void_t => "void" | Label_t => "label"
+      | X86mmx_t => "x86mmx" | Metadata_t => "metadata"
+      | Array_t ns t => 
+        List.fold_right (fun (i:nat) (t:string) => 
+                         "[" ++ (string_of_nat i) ++ " x " ++ t ++ "]") (string_of_type t) ns
+      | Fn_t t ts vararg => 
+        (string_of_type t) ++ "(" ++ (sep ", " (List.map string_of_type ts)) ++ 
+        (if vararg then ",...)" else ")")
+      | Struct_t packed elts => 
+        let s := "{" ++ (sep ", " (List.map string_of_type elts)) ++ "}" in 
+          if packed then "<" ++ s ++ ">" else s
+      | Named_t x => x
+      | Opaque_t => "opaque"
+      | Pointer_t 0 t => (string_of_type t) ++ " *"
+      | Pointer_t n t => (string_of_type t) ++ "addrspace(" ++ (string_of_nat n) ++ ") *"
+      | Vector_t n t => "<" ++ (string_of_nat n) ++ " x " ++ (string_of_type t) ++ ">"
+    end.
+
+  Fixpoint string_of_constant (c:constant) : string := 
+    match c with 
+      | True_c => "true" | False_c => "false" 
+      | Int_c i => string_of_Z i
+      | Float_c s => s | Null_c =>  "null" | Global_c v => v 
+      | Undef_c => "undef" | Zero_c => "zeroinitializer"
+      | Struct_c cs => "{" ++ (sep ", " (List.map string_of_constant cs)) ++ "}"
+      | Array_c cs => "[" ++ (sep ", " (List.map string_of_constant cs)) ++ "]"
+      | Vector_c cs => "<" ++ (sep ", " (List.map string_of_constant cs)) ++ ">"
+      | Metastring_c s => "!" ++ (quoted s)
+      | Metadata_c cs => "!{" ++ (sep ", " (List.map string_of_constant cs)) ++ "}"
+    end.
+
+  Definition string_of_value(v:value) : string := 
+    match v with 
+      | Local x => "%" ++ x
+      | Global x => "@" ++ x
+      | AnonLocal n => "%" ++ (string_of_nat n)
+      | AnonGlobal n => "@" ++ (string_of_nat n)
+      | Constant c => string_of_constant c
+    end.
+
+  Definition string_of_cond(c:cond) : string := 
+    match c with 
+      | Eq => "eq" | Ne => "ne" | Ugt => "ugt" | Uge => "uge" | Ult => "ult" | Ule => "ule" 
+      | Sgt => "sgt" | Sge => "sge" | Slt => "slt" | Sle => "sle"
+    end.
+
+  Definition string_of_fcond(f:fcond) : string := 
+    match f with 
+      | False_fc => "false" | Oeq_fc => "oeq" | Ogt_fc => "ogt" | Oge_fc => "oge" | Olt_fc => "olt"
+      | Ole_fc => "ole" | One_fc => "one" | Ord_fc => "ord" | Ueq_fc => "ueq" | Ugt_fc => "ugt"
+      | Uge_fc => "uge" | Ult_fc => "ult" | Ule_fc => "ule" | Une_fc => "une" | Uno_fc => "uno"
+      | True_fc => "true"
+    end.
 
   Definition string_of_arith(opcode:string)(nuw nsw:bool)(ty:type)(op1 op2:value) : string := 
     opcode ++ " " ++ (flag nuw "nuw ") ++ (flag nsw "nsw ") ++ (string_of_type ty) ++ " " ++ 
@@ -354,18 +510,6 @@ Module LLVM.
                                       end) args)) 
         ++ ") " ++ (sep " " (List.map string_of_fn_attr fnattrs))
     end.
-  
-  Inductive instr : Type := 
-  | Comment_i : string -> instr
-  | Ret_i : option (type * value) -> instr
-  | Br_cond_i : value -> label -> label -> instr
-  | Br_uncond_i : label -> instr
-  | Switch_i : type -> value -> label -> list (type * Z * label) -> instr
-  | Resume_i : type -> value -> instr
-  | Unreachable_i : instr
-  | Assign_i : (option value) -> exp -> instr
-  | Store_i : forall (atomic:bool) (volatile:bool) (ty:type) (v:value) (ptrty:type) (pointer:value) 
-                     (align:option nat) (nontemporal:option nat) (singlethread:bool), instr.
 
   Definition string_of_instr(i:instr) : string := 
     match i with 
@@ -395,152 +539,12 @@ Module LLVM.
         (string_of_option (fun n => ", align "++(string_of_nat n)++" ") align)
     end.
 
-  Definition ST := state (list string).
-  Definition emit : string -> ST unit := CPS.emit.
-  Definition spaces (n:nat) : ST unit := emit (CPS.spaces n).
-  Definition newline : ST unit := emit CPS.newline.
-
-  Section SEPBY.
-    Variable A : Type.
-    Variable f : A -> ST unit.
-    Variable sep : ST unit.
-
-    Fixpoint sepby (xs:list A) : ST unit :=
-      match xs with
-        | nil => ret tt
-        | h::nil => f h
-        | h::t => f h ;; sep ;; sepby t
-      end.
-  End SEPBY.
-
-  Definition iter := @CPS.iter.
-  Definition emit_option {A} (f:A -> ST unit) (x:option A) : ST unit := 
-    match x with 
-      | None => ret tt
-      | Some v => f v 
-    end.
-  Definition emit_option_s {A} (f:A -> ST unit) (x:option A) : ST unit := 
-    match x with 
-      | None => ret tt
-      | Some v => f v ;; emit " "
+  Fixpoint sep (s:string) (ss:list string) : string := 
+    match ss with 
+      | nil => ""
+      | h::nil => h
+      | h::t => h ++ s ++ (sep s t)
     end.
 
-  Definition emit_instr (i:instr) : state (list string) unit := 
-    spaces 4 ;; emit (string_of_instr i) ;; newline.
 
-  Definition block := ((option label) * (list instr))%type.
-
-  Definition emit_block (b:block) : state (list string) unit := 
-    emit_option (fun l => spaces 2 ;; emit l ;; emit ":" ;; newline) (fst b) ;; 
-    iter emit_instr (snd b).
-
-  Definition pipe {A B C} (f:B -> C) (g:A -> B) : A -> C := 
-    fun x => f (g x).
-
-  Infix "$" := pipe (at level 70, right associativity).
-
-  Record fn_header : Type := {
-    linkage_fh : option linkage ; 
-    visibility_fh : option visibility ; 
-    cconv_fh : option cconv ; 
-    unnamed_addr_fh : bool ; 
-    return_type_fh : type ; 
-    return_type_attrs_fh : list param_attr ; 
-    name_fh : var ; 
-    args_fh : list (type * var * list (param_attr)) ; 
-    attrs_fh : list fn_attr ; 
-    section_fh : option string ; 
-    align_fh : option nat ; 
-    gc_fh : option string
-  }.
-
-  Definition emit_fn_header (drop_vars:bool) (fh:fn_header) : state (list string) unit := 
-    emit_option_s (emit $ string_of_linkage) (linkage_fh fh) ;; 
-    emit_option_s (emit $ string_of_visibility) (visibility_fh fh) ;; 
-    emit_option_s (emit $ string_of_cconv) (cconv_fh fh) ;;
-    (if (unnamed_addr_fh fh) then emit "unnamed_addr " else ret tt) ;; 
-    emit (string_of_type (return_type_fh fh)) ;; emit " " ;;
-    iter (fun x => emit (string_of_param_attr x) ;; emit " ") (return_type_attrs_fh fh) ;;
-    emit "@" ;; emit (name_fh fh) ;; emit "(" ;; 
-    sepby (fun p => match p with (t,x,attrs) => 
-                     emit (string_of_type t) ;; 
-                     (if drop_vars then ret tt else emit " %"%string ;; emit x) ;;
-                     iter (fun x => emit (string_of_param_attr x) ;; emit " ") attrs
-                   end) (emit ", ") (args_fh fh) ;;
-    emit ") " ;;
-    iter (fun x => emit (string_of_fn_attr x) ;; emit " ") (attrs_fh fh) ;;
-    emit_option_s (fun s => emit ", section " ;; emit (quoted s) ;; emit " ") (section_fh fh) ;;
-    emit_option_s (fun n => emit ", align " ;; emit (string_of_nat n) ;; emit " ") (align_fh fh) ;;
-    emit_option_s (fun s => emit "gc " ;; emit (quoted s) ;; emit " ") (gc_fh fh).
-    
-  Inductive topdecl : Type := 
-  | Global_d : forall (x:var) (addrspace:option nat) (l:option linkage) (unnamed_addr:bool) (const:bool) 
-                      (t:type) (c:constant) (section:option string) (align:option nat), topdecl
-  | Define_d : fn_header -> list block -> topdecl
-  | Declare_d : fn_header -> topdecl
-  | Alias_d : forall (x:var) (l:option linkage) (v:option visibility) (t:type) (e:exp), topdecl
-  | Metadata_d : forall (x:var), list constant -> topdecl.
-
-  Definition emit_topdecl (t:topdecl) : ST unit := 
-    match t with 
-      | Global_d x a l u c t v s al => 
-        emit x ;; emit " = " ;;
-        emit_option_s (fun n => emit "addrspace(" ;; emit (string_of_nat n) ;; emit ")") a ;;
-        emit_option_s (emit $ string_of_linkage) l ;;
-        (if u then emit "unnamed_addr " else ret tt) ;;
-        (if c then emit "constant " else ret tt) ;;
-        emit (string_of_type t) ;; emit " " ;; 
-        emit (string_of_constant v) ;; emit " " ;;
-        emit_option_s (fun s => emit ", section " ;; emit (quoted s) ;; emit " ") s ;;
-        emit_option_s (fun n => emit ", align " ;; emit (string_of_nat n) ;; emit " ") al ;;
-        newline 
-      | Define_d fh bs => emit "define " ;;
-        emit_fn_header false fh ;; emit " {" ;; newline ;; iter emit_block bs ;; emit "}" ;; newline
-      | Declare_d fh => emit "declare " ;; emit_fn_header true fh ;; newline
-      | Alias_d x l v t e => 
-        emit x ;; emit " = alias " ;; 
-        emit_option_s (emit $ string_of_linkage) l ;;
-        emit_option_s (emit $ string_of_visibility) v ;;
-        emit (string_of_type t) ;; emit " " ;; 
-        emit (string_of_exp e) ;; newline
-      | Metadata_d x cs => 
-        emit x ;; emit " = metadata !{" ;; emit (sep ", " (List.map string_of_constant cs)) ;; 
-        emit "}" ;; newline
-    end.
-
-  Definition module := list topdecl.
-
-  Definition emit_module (m:module) : ST unit := iter emit_topdecl m.
-
-  Definition runST (c:ST unit) := 
-    List.fold_left (fun x y => y ++ x) (snd (runState c nil)).
-
-  Definition string_of_module := runST $ emit_module.
-  Definition string_of_topdecl := runST $ emit_topdecl.
-  Definition string_of_fn_header b := runST $ (emit_fn_header b).
-
-  (* 
-  Definition test_block : block := (None, Comment_i "Here is a comment." :: Ret_i None :: nil).
-  Definition test : topdecl :=
-    Define_d
-    {|
-      linkage_fh := None;
-      visibility_fh := None;
-      cconv_fh := None;
-      unnamed_addr_fh := false;
-      return_type_fh := I_t 3;
-      return_type_attrs_fh := nil;
-      name_fh := "test";
-      args_fh := nil;
-      attrs_fh := nil;
-      section_fh := None;
-      align_fh := None;
-      gc_fh := None |} 
-    (test_block :: nil).
-
-  Eval compute in (string_of_topdecl test "").
-  *)
-
-
-End LLVM.
-
+*)
